src/3d/Options.fsti
@@ -1,6 +1,8 @@
 module Options
 open FStar.All
 
+type check_hashes_t = | NoHashes | WeakHashes | StrongHashes
+
 val display_usage : unit -> ML unit
 
 val parse_cmd_line : unit -> ML (list string)
@@ -26,3 +28,7 @@ val get_cleanup : unit -> ML bool
 val get_skip_makefiles : unit -> ML bool
 
 val get_no_everparse_h : unit -> ML bool
+
+val get_check_hashes : unit -> ML check_hashes_t
+
+val get_save_hashes : unit -> ML bool
