src/3d/Batch.fsti
@@ -6,6 +6,8 @@ val postprocess
   (clang_format_executable: string)
   (cleanup: bool)
   (no_everparse_h: bool)
+  (check_weak_hashes: option bool)
+  (save_hashes: bool)
   (out_dir: string)
   (files_and_modules: list (string & string))
 : ML unit
